Fix an issue with EIP-6780 implementation
This might not be completely fixed yet, but there are subtleties
regarding accounts that are created that were not empty before the
transaction.

spec/prop/vfmComputeScript.sml
@@ -615,6 +615,18 @@ val () = “ensure_storage_in_domain x s” |>
     COND_RATOR, LET_RATOR
   ] |> cv_auto_trans;
 
+val set_original_pre_def = “set_original a s” |>
+  SIMP_CONV std_ss [
+    set_original_def
+  ] |> cv_auto_trans_pre;
+
+Theorem set_original_pre[cv_pre]:
+  set_original_pre a s
+Proof
+  rw[set_original_pre_def]
+  \\ Cases_on`s` \\ gs[]
+QED
+
 (*
   set_goal([], pre_a)
 *)
